proof/agp32_WB_CorrectScript.sml
@@ -1,0 +1,30 @@
+open hardwarePreamble translatorTheory translatorLib arithmeticTheory wordsExtraTheory dep_rewrite blastLib bitstringSyntax fcpSyntax listSyntax wordsSyntax agp32StateTheory agp32EnvironmentTheory agp32ProcessorTheory ag32Theory ag32ExtraTheory ag32UtilitiesTheory agp32RelationTheory agp32UpdateTheory agp32InternalTheory;
+
+(* correctness of WB stage items with respect to the ISA *)
+val _ = new_theory "agp32_WB_Correct";
+
+val _ = prefer_num ();
+val _ = guess_lengths ();
+
+
+(* registers R updated by WB stage *)
+Theorem agp32_Rel_ag32_R_correct:
+  !fext fbits a t I.
+    is_sch I (agp32 fext fbits) a ==>
+    Rel I (fext t) (agp32 fext fbits (t-1)) (agp32 fext fbits t) a t ==>
+    I (5,t) <> NONE ==>
+    reg_data_vaild 5 (agp32 fext fbits t) ==>
+    (agp32 fext fbits (SUC t)).R = (FUNPOW Next (THE (I (5,t))) a).R
+Proof
+  rw [] >> Q.ABBREV_TAC `s = agp32 fext fbits t` >>
+  Q.ABBREV_TAC `s' = procs [agp32_next_state;WB_pipeline;MEM_pipeline;EX_pipeline] (fext t) s s` >>
+  `(agp32 fext fbits (SUC t)).R = (REG_write (fext t) s s').R` by cheat >>
+  fs [REG_write_def,reg_data_vaild_def] >>
+  `(s'.R = s.R) /\ (s'.WB.WB_state_flag <=> s.WB.WB_state_flag) /\
+  (s'.WB.WB_write_data = s.WB.WB_write_data)` by cheat >> fs [] >>
+  Cases_on `s.WB.WB_write_reg` >> fs [] >-
+   (fs [Rel_def] >> cheat) >>
+  cheat
+QED
+
+val _ = export_theory ();
